<?xml version="1.0" encoding="UTF-8"?>

<appendix xml:id="algebrareview" xmlns:xi="http://www.w3.org/2001/XInclude">
	<title>Algebra Review</title>
	
	<section xml:id="sec_algebralaw">
		<title>Laws of Algebra</title>
		
		<assemblage xml:id="assemblage-distributing">
			<title>Distributing and FOIL-ing</title>
			<p>
				Distribute <m>a</m> to all terms: 
					<me> a \cdot (b+c) = a\cdot b + a \cdot c</me>
				The best way to remember this is by drawing arcs from <m>a</m> to <m>b</m> and <m>c</m>
			</p>
			<image xml:id="img_distribute" width="20%">
				
				<latex-image>
					%% Code taken from stackexchange
					\begin{tikzpicture}
					
						\node[anchor=base,text height = 8pt] (a)  at (0,0) {$a$}; 
						\node[anchor=base,text height = 8pt] (op) at (1em,0) {(};
						\node[anchor=base,text height = 8pt] (b)  at (2em,0) {$b$};
						\node[anchor=base,text height = 8pt] (+)  at (3em,0) {$+$};
						\node[anchor=base,text height = 8pt] (c)  at (4em,0) {$c$};
						\node[anchor=base,text height = 8pt] (cp) at (5em,0) {)};

						\draw[thick,red] (a.north) to [out=45, in=135] (b.north);
						\draw[thick,blue] (a.north) to [out=60, in=120] (c.north);
						
					\end{tikzpicture}
				</latex-image>
			</image>

			<p>
				FOIL the expression: 
					<me>(a + b) \cdot (c + d) = (a\cdot c) + (a \cdot d) + (b\cdot c) + (b\cdot d)</me>
			</p>
			<p>
				The best way to remember this formula is by drawing arcs from <m>a</m> and <m>b</m> to <m>c</m> and <m>d</m>.
			</p>
			<image xml:id="img_foil" width="40%">
				
				<latex-image>
					%% Code taken from stackexchange
					\begin{tikzpicture}
						\node[anchor=base,text height = 8pt] at (0em,0) {(};
						\node[anchor=base,text height = 8pt] (a) at (1em,0) {$a$};
						\node[anchor=base,text height = 8pt] at (2em,0) {$+$};
						\node[anchor=base,text height = 8pt] (b) at (3em,0) {$b$};
						\node[anchor=base,text height = 8pt] at (4em,0) {)};
						\node[anchor=base,text height = 8pt] at (5em,0) {$\cdot$};
						\node[anchor=base,text height = 8pt] at (6em,0) {(};
						\node[anchor=base,text height = 8pt] (c) at (7em,0) {$c$};
						\node[anchor=base,text height = 8pt] at (8em,0) {$+$};
						\node[anchor=base,text height = 8pt] (d) at (9em,0) {$d$};
						\node[anchor=base,text height = 8pt] at (10em,0) {)};

						\draw[thick,red] (a.north) to [out=45, in=135] (c.north);
						\draw[thick,blue] (a.north) to [out=60, in=120] (d.north);
						\draw[thick,red] (b.south) to [out=-45, in=-135] (c.south);
						\draw[thick,blue] (b.south) to [out=-60, in=-120] (d.south);
						
					\end{tikzpicture}
				</latex-image>
			</image>
		</assemblage>

		<example>
			<title>Understanding FOIL-ing</title>
			
			<p>
				The mathematical expression for simplifying <m>(a+b)\cdot(c+d)</m> can look a bit mysterious.  To understand why it looks the way it does, it is helpful to remember the connection between multiplication and area.
			</p>
			<p>
				For example, if you have a rectangle of side lengths <m>5</m> and <m>2</m>, then the rectangle has area <m>5\cdot 2 = 10</m>.  Visually, we have the following picture.
			</p>
			<image xml:id="img_multarea" width="33%">
				
				<latex-image>
					\begin{tikzpicture}
						\node[below] (BO) at (0,0) {};
						\node[left] (LO) at (0,0) {};
						\node[below] (BM) at (5,0) {};
						\node[left] (LM) at (0,2) {};
						\draw (0,0) rectangle (5,2);
						\draw[dimen] (BO.south) -- (BM.south) node [midway,below] {$5$};
						\draw[dimen] (LO.west) -- (LM.west) node [midway,left] {$2$};
						\node at (2.5,1) {$2\cdot 5 = 10$};
					\end{tikzpicture}
				</latex-image>
			</image>
			<p>
				Suppose instead we increase the lengths of the sides to <m>8=5+3</m> and <m>6 = 2+4</m>.  Let's see how this changes our area. 
			</p>
			<image xml:id="img_multareasum" width="66%">
				
				<latex-image>
					\begin{tikzpicture}
						\node[below] (BO) at (0,0) {};
						\node[left] (LO) at (0,0) {};
						\node[below] (BM) at (5,0) {};
						\node[left] (LM) at (0,2) {};
						\node[below] (BE) at (8,0) {};
						\node[left] (LE) at (0,6) {};
						\draw (0,0) rectangle (8,6);
						\draw (5,0) -- (5,6);
						\draw (0,2) -- (8,2);
						\draw[dimen] (BO.south) -- (BM.south) node [midway,below] {$5$};
						\draw[dimen] (BM.south) -- (BE.south) node [midway,below] {$3$};
						\draw[dimen] (LM.west) -- (LE.west) node [midway,left] {$4$};
						\draw[dimen] (LO.west) -- (LM.west) node [midway,left] {$2$};
						\node at (2.5,1) {$2\cdot 5 = 10$};
						\node at (6.5,1) {$2\cdot 3 = 6 $};
						\node at (2.5,4) {$4\cdot 5 = 20$};
						\node at (6.5,4) {$4\cdot 3 = 12$};
					\end{tikzpicture}
				</latex-image>
			</image>
			<p>
				The area given by <m>(5+3)\cdot(2+4)</m> has four regions, each with their own area
				<me>
					5\cdot 2 + 5\cdot 4 + 3 \cdot 2 + 3\cdot 4
				</me>
			</p>
			<p>
				The same mathematical pattern occurs when you have variables in your side lenghts.  Suppose you have a rectangle with one side <m>3x + 2</m> and another side <m>x+5</m>.  Then the area of the rectangle still has four regions 
			</p>
			<image xml:id="img_multareapoly" width="66%">
				
				<latex-image>
					\begin{tikzpicture}
						\node[below] (BO) at (0,0) {};
						\node[left] (LO) at (0,0) {};
						\node[below] (BM) at (5,0) {};
						\node[left] (LM) at (0,2) {};
						\node[below] (BE) at (8,0) {};
						\node[left] (LE) at (0,6) {};
						\draw (0,0) rectangle (8,6);
						\draw (5,0) -- (5,6);
						\draw (0,2) -- (8,2);
						\draw[dimen] (BO.south) -- (BM.south) node [midway,below] {$3x$};
						\draw[dimen] (BM.south) -- (BE.south) node [midway,below] {$2$};
						\draw[dimen] (LM.west) -- (LE.west) node [midway,left] {$5$};
						\draw[dimen] (LO.west) -- (LM.west) node [midway,left] {$x$};
						\node at (2.5,1) {$3x\cdot x = 3x^2 $};
						\node at (6.5,1) {$2\cdot x = 2x $};
						\node at (2.5,4) {$3x\cdot 5 = 15x$};
						\node at (6.5,4) {$2\cdot 5 = 10$};
					\end{tikzpicture}
				</latex-image>
			</image>
			<p>
				Adding up the areas of those regions gives us the same thing as FOIL-ing
				<me>
					(3x+2)(x+5) = (3x\cdot x) + (3x\cdot 5) + (2\cdot x) + (2\cdot 5)
				</me>
				Simplifying that down we get
				<me>
					(3x+2)(x+5) = 3x^2 + 17x + 10
				</me>
				Of course, with practice, it is faster and easier to learn to use the formula for FOIL-ing than would be to go through the area derivation each time.  
			</p>
		</example>

		<exploration xml:id="ex-review-distributefactor">
			<introduction>
				<p>
					Use the laws of algebra listed above to simplify the following expressions completely. 
				</p>
			</introduction>
			<task>
				<statement>
					<p>
						<m>5(x^2 - 3x + 2)</m>
					</p>
				</statement>
				<solution>
					<p>
						We must distribute the 5 to every term of the expression
						<md>
							<mrow> 5(x^2 - 3x + 2) \amp = 5x^2 - 15 x  + 10 </mrow>
						</md>
					</p>
				</solution>
			</task>
			<task>
				<statement>
					<p>
						<m>(-1)(x - 5)</m>
					</p>
				</statement>
				<solution>
					<p>
						We must distribute a <m>-1</m> to each term
						<md>
							<mrow> (-1)(x - 5)	\amp = (-1)x - (-1)5 </mrow>
							<mrow> \amp = -x + 5</mrow>
						</md>
					</p>
				</solution>
			</task>
			<task>
				<statement>
					<p>
						<m>(x+6)(x-2)</m>
					</p>
				</statement>
				<solution>
					<p>
						We must foil the expression using the formula 
						<me>
							(a + b) \cdot (c + d) = (a\cdot c) + (a \cdot d) + (b\cdot c) + (b\cdot d)
						</me>
						with <m>a=x</m>, <m>b=6</m>, <m>c=x</m>, and <m>d=-2</m>.
						In other words, we have 
							<md>
								<mrow> (x+6)(x-2)\amp = (x\cdot x) + (x\cdot -2)+ (6\cdot x) + (6\cdot -2)</mrow>
								<mrow> \amp = x^2 - 2x + 6x - 12 \amp </mrow>
								<mrow> \amp = x^2 + 4x - 12</mrow>
							</md>
						</p>

				</solution>
			</task>
			<task>
				<statement>
					<p>
						<m>(5x-1)(2x+1)</m>
					</p>
				</statement>
				<solution>
					<p>
						We must foil the expression using the formula 
						<me>
							(a + b) \cdot (c + d) = (a\cdot c) + (a \cdot d) + (b\cdot c) + (b\cdot d)
						</me>
						with <m>a=5x</m>, <m>b=-1</m>, <m>c=2x</m>, and <m>d=1</m>.
						In other words, we have 
							<md>
								<mrow> (5x-1)(2x+1)\amp = (5x\cdot 2x) + (5x\cdot 1)+ (-1\cdot 2x) + (-1\cdot 1)</mrow>
								<mrow> \amp = 10x^2 + 5x - 2x - 1 \amp </mrow>
								<mrow> \amp = 10x^2 + 3x - 1</mrow>
							</md>
						</p>

				</solution>
			</task>
			<task>
				<statement>
					<p>
						<m>(2x+3)^2</m>
					</p>
				</statement>
				<solution>
					<p>
						Squaring an expression means multipling it by itself twice. In other words, 
						<md>
							<mrow> (2x+3)^2 \amp = (2x+3)\cdot (2x+3)</mrow>
							<mrow> \amp = (2x\cdot 2x) + (2x\cdot 3) + (3\cdot 2x) + (3\cdot 3)</mrow>
							<mrow> \amp = 4x^2 + 6x + 6x + 9</mrow>
							<mrow> \amp = 4x^2 + 12x + 9</mrow>
						</md>
					</p>
				</solution>
			</task>
			<task>
				<statement>
					<p>
						<m>(-3)(2x+3)^2</m>
					</p>
				</statement>
				<solution>
					<p>
						We must use order of operations to decide which operation to perform first.  Remember that PEMDAS (parentheses, exponents, multiplcation/division, addition/subtraction) tells us which operations attach more "strongly", and must be performed first.  
						<ol>
							<li>
								<p>
									Here, the parentheses group the expression into two parts: <m>A\cdot B^2</m> with <m>A=(-3)</m> and <m>B=(2x+3)</m>.  
								</p>
							</li>
							<li>
								<p>
									Exponentiation is stronger than multiplication, so we must first square <m>(2x+3)</m>.  As in the previous problem, we have
									<md>
										<mrow> (-3)(2x+3)^2\amp = (-3)\cdot (4x^2 + 12x + 9) </mrow>
									</md>
								</p>
							</li>
							<li>
								<p>
									Now, we can distribute <m>-3</m> to each term. 
									<md>
										<mrow> \amp = (-3)\cdot (4x^2 + 12x + 9) </mrow>
										<mrow> \amp = (-3\cdot 4) x^2+ (-3\cdot 12)x + (-3\cdot 9)</mrow>
										<mrow> \amp = -12x^2 - 36x - 27</mrow>
									</md>
								</p>
							</li>
						</ol>
					</p>
				</solution>
			</task>
			<task>
				<statement>
					<p>
						Factor the following expression as much as possible
						<m>9x - 15</m>
					</p>
				</statement>
				<solution>
					<p>
						First, factor each term in the expression. There is a 3 in each term, so we can factor it out. 
						<md>
							<mrow>9x - 15 \amp = (3\cdot 3)x - (3\cdot 5) </mrow>
							<mrow> \amp = 3 (3x - 5)</mrow>
						</md>
						There are no remaining common terms, so we are done factoring. 
					</p>
				</solution>
			</task>
			<task>
				<statement>
					<p>
						Factor the following expression as much as possible
						<m>x^2 + x - 6 </m>
					</p>
				</statement>
				<solution>
					<p>
						We want to write <m>x^2 + x - 6 </m> as an expression of the form <m>(a x + b) (c x + d) </m>
						<me>
							(a x + b) (c x + d)  = (ab)x^2 + (ad+cb)x + bd
						</me>
						We want to pick <m>a,b,c,d</m> to get the right hand side to equal <m>x^2+x-6</m>. 
						There are three terms to consider
						<ul>
							<li> 
								<p>
									We need <m>(ab)x^2=x^2</m>, so set <m>a=b=1</m>.
									Plugging that into our factored form, we get
									<me>
										(x + b)(x+d) = x^2 + (d+b)x + bd 
									</me>
								</p>
							</li>
							<li>
								<p>
									We need the third term to be <m>db=-6</m>.  Factoring gives <m>db = (-1)\cdot 2\cdot 3</m>.  We must divide the factors <m>-1</m>, <m>2</m>, <m>3</m> between <m>b,d</m>.  
								</p>
							</li>
							<li>
								<p>
									To pick exact values for <m>b,d</m>, recall that we need <m>b+d=1</m>. Setting <m>b=3</m> and <m>d=(-1)2</m>, we can confirm
									<md>
										<mrow>bd \amp = (3)(-1)(2) = -6</mrow>
										<mrow>b+d \amp = 3 + (-1)(2) = 1</mrow>
									</md>
									as desired.
								</p>
							</li>
						</ul>
						Putting it together, we get 
						<md>
							<mrow>x^2 + x - 6 \amp = (x+3)(x-2) </mrow>
						</md>
					</p>
				</solution>
			</task>
			<task>
				<statement>
					<p>
						Factor the following expression as much as possible
						<m>2x^7 + 5x^3 </m>
					</p>
				</statement>
				<solution>
					<p>
						First, factor each term in the expression. There are three occurances of <m>x</m> in each term, so we can factor them out. 
						<md>
							<mrow>2x^7 + 5x^3 \amp = (2\cdot x \cdot x\cdot x\cdot x\cdot x\cdot x\cdot x) + (5\cdot x\cdot x\cdot x) </mrow>
							<mrow> \amp = x\cdot x\cdot x (2\cdot x\cdot x\cdot x\cdot x + 5)</mrow>
							<mrow> \amp = x^3 (2 x^4 + 5)</mrow>
						</md>
						There are no remaining common terms, so we are done factoring. 
					</p>
				</solution>
			</task>
		</exploration>

		<axiom xml:id="fraction-arithmetic">
			<title>Laws of Fractions</title>
			
			<statement>
				<p>
					Suppose that <m>b,e\neq 0</m>
				</p>
				<sidebyside margins="10%">
					<ul marker="circle">
						<li>
							<m>\frac{a}{b} + \frac{c}{d} = \frac{ad + cb}{bd}</m>
						</li>
						<li>
							<m> \frac{a}{b} + \frac{c}{b}=  \frac{a+c}{b}</m>
						</li>
						<li>
							<m> \frac{a}{b} \cdot \frac{c}{e} =  \frac{a\cdot c}{b\cdot e}</m>
						</li>
						<li>
							<!--m> \frac{a}{b}=  \frac{a\cdot e}{b\cdot e}</m-->
							<m>  \frac{a\cdot e}{b\cdot e} = \frac{a}{b}</m>
						</li>
					</ul>
					<ul marker="circle">
						<li>
							<m> \frac{a}{b} - \frac{c}{b} =  \frac{a-c}{b}</m>
						</li>
						<li>
							<m> \frac{1}{\ \frac{b}{e}\ }=  \frac{e}{b}</m>
						</li>
						<li>
							<m> a\cdot \frac{c}{b}=  \frac{a\cdot c}{b}</m>
						</li>
					</ul>
				</sidebyside>
			</statement>

		</axiom>

		<exploration xml:id="ex-review-fractionlaws">
			<introduction>
				<p>
					Use the laws of algebra listed above to simplify the following expressions completely. 
				</p>
			</introduction>
			<task>
				<statement>
					<p>
						<m>\dfrac{ab - a}{b-1}</m>
					</p>
				</statement>
				<solution>
					<p>
						<me>
							\dfrac{ab - a}{b-1} = \dfrac{a(b-1)}{1\cdot (b-1)} = \dfrac{a}{1}
						</me>
						
					</p>
				</solution>
			</task>
			<task>
				<statement>
					<p>
						Simplify <m>\dfrac{a-b}{b-a}</m>
					</p>
				</statement>
				<solution>
					<p>
						<md>
							<mrow>\dfrac{a-b}{b-a} \amp = \dfrac{a-b}{-a + b }</mrow>
							<mrow> \amp = \dfrac{a-b}{(-1) ( a - b)}</mrow>
							<mrow> \amp = \dfrac{1}{-1}</mrow>
							<mrow> \amp = -1</mrow>
						</md>
					</p>
				</solution>
			</task>
		</exploration>



		<axiom xml:id="exponential-arithmetic">
			<title>Laws of Exponents</title>
			<statement>
				<p>
					Let <m>a,b&gt; 0</m> in the following.
				</p>
				<sidebyside margins="10%">
						<ul marker="circle">
							<li>
								<m> \sqrt[r]{a}=  a^{1/r}</m>
							</li>
							<li>
								<m> a^{r+s} =  a^r\cdot a^s </m>
							</li>
							<li>
								<m> {\left(a^{r}\right)}^s=  a^{r\cdot s}</m>
							</li>
							<li>
								<m> {\left(a\cdot b\right)}^{r}=  a^{r}\cdot b^{r}</m>
							</li>
							<li>
								<m> \sqrt[r]{a\cdot b}=  \sqrt[r]{a}\cdot \sqrt[r]{b}</m>
							</li>
						</ul>
						<ul marker="circle">
							<li>
								<m> a^{r-s}=  \frac{a^r}{a^s}</m>
							</li>
							<li>
								<m> a^{-s}=  \frac{1}{a^s}</m>
							</li>
							<li>
								<m> a^{s}=  \frac{1}{a^{-s}}</m>
							</li>
							<li>
								<m> \frac{1}{a^{s}} =  \left(\frac{1}{a}\right)^s</m>
							</li>
						</ul>
				</sidebyside>
			</statement>
		</axiom>

		
		
		
		
		
		

		<example xml:id="fractions-which-do-not-simplify-easily" >
			<title>Fractions which do NOT simplify easily</title>

			<p>
				Doesn't simplify at all: <m>\dfrac{3}{x+1}</m>
			</p>

			<p>
				Must find a common denomiator before you can combine terms: <me>\dfrac{x+1}{x-1} + \dfrac{1}{x} = \dfrac{\,x\cdot (x+1) + (x-1)\cdot 1\,}{x\cdot (x-1)} = \dfrac{x^2+2x-1}{x^2-x}</me>
			</p>

		</example>

		<example xml:id="exponents-and-products-that-do-not-simplify-easily" >
			<title>Exponents and Products that do NOT simplify easily</title>

			<p>
				Doesn't simplify at all: <m>\sqrt{x+1} = (x+1)^{1/2}</m>
			</p>

			<p>
				You must FOIL to simplify: <m>(x+1)^2 = (x+1)(x+1) = x^2 + 2x + 1</m>
			</p>

		</example>
	</section>

	
	<section xml:id="sec-IntervalsandGraphs">
		<title>Intervals and Graphs</title>

		<subsection xml:id="interval-notation">
			<title>Interval Notation</title>

			<p>
				When using <em>interval notation</em> to represent sets, square brackets include the endpoint and parentheses exclude the endpoint. Multiple intervals can be combined using <m>\cup</m> (or U).
			</p>

			<p><ul>
				<li>
								<p>
				<m>[-1,1)</m> represents the numbers <m>x</m> such that <m>-1\leq x &lt;1</m>. 
			</p>

				<image width="50%" xml:id="img_intervals1"> 
					
					<latex-image>
						\begin{tikzpicture}
							\foreach \i in {-2,...,2}
							{
								\draw (\i,-1mm)--(\i,1mm);
								\node[below] at (\i,-1mm) {\i};
								\node[above] at (\i,1mm){$\phantom{\i}$};
							}
							\draw[latex-latex] (-3,0) -- (3,0);
							\draw[ultra thick] (-1,0) -- (1,0);
							\draw[fill=black] (-1,0) circle (3pt);
							\draw[fill=white] (1,0) circle (3pt);
						\end{tikzpicture}
					</latex-image>
				</image>
				</li>

				<li>
								<p>
				<m>[0,\infty)</m> represents the numbers <m>x</m> such that <m>0\leq x </m>.
			</p>

				<image width="50%" xml:id="img_intervals2">
					
					<latex-image>
						\begin{tikzpicture}
							\foreach \i in {-2,...,2}
							{
								\draw (\i,-1mm)--(\i,1mm);
								\node[below] at (\i,-1mm) {\i};
								\node[above] at (\i,1mm){$\phantom{\i}$};
							}
							\draw[latex-latex] (-3,0) -- (3,0);
							\draw[ultra thick,-latex] (0,0) -- (3,0);
							\draw[fill] (0,0) circle (3pt);
						\end{tikzpicture}
					</latex-image>
				</image>
				</li>

				<li>
								<p>
				<m>(-\infty,-1)\bigcup (1,2]</m> represents the numbers <m>x</m> such that <em>either</em> <m>x&lt;-1</m> <em>or</em> <m>1&lt;x\leq 2</m>.
			</p>

				<image width="50%" xml:id="img_intervals3">
					
					<latex-image>
						\begin{tikzpicture}
							\foreach \i in {-2,...,2}
							{
								\draw (\i,-1mm)--(\i,1mm);
								\node[below] at (\i,-1mm) {\i};
								\node[above] at (\i,1mm){$\phantom{\i}$};
							}
							\draw[latex-latex] (-3,0) -- (3,0);
							\draw[ultra thick,&lt;-] (-3,0) -- (-1,0);
							\draw[ultra thick] (1,0) -- (2,0);
							\draw[fill=white] (-1,0) circle (3pt);
							\draw[fill=white] (1,0) circle (3pt);
							\draw[fill=black] (2,0) circle (3pt);
						\end{tikzpicture}
					</latex-image>
				</image>
				</li>

			</ul></p>

		</subsection>

		<subsection xml:id="graphs-of-common-functions" >
			<title>Graphs of Common Functions</title>

				<image width="50%" xml:id="img_graphs1">
					
					<latex-image>
							\begin{tikzpicture}[scale=1]
								%\draw[step=.5cm,grid] (-2.4,-2.4) grid (2.4,2.4);
								\draw[axes] (-2.4,0) -- (2.4,0);
								\draw[axes] (0,-2.4) -- (0,2.4);		
								%%
								\draw [curve,smooth,samples=100,domain=-1.4:1.4] plot (\x, \x*\x);
								\node at (-2.5,1) {$f(x)= x^2$};
								%%
								\draw [curve,dashed,samples=100,domain=-1.3:1.3] plot (\x, \x*\x*\x);
								\node at (-2.5,-1) {$f(x)= x^3$};
							\end{tikzpicture}
					</latex-image>
				</image>
				<image width="50%" xml:id="img_graphs2">
					
					<latex-image>
							\begin{tikzpicture}[scale=1]
								%\draw[step=.5cm,grid] (-2.4,-2.4) grid (2.4,2.4);
								\draw[axes] (-2.4,0) -- (2.4,0);
								\draw[axes] (0,-2.4) -- (0,2.4);		
								%%
								\draw [curve,smooth,samples=100,domain=0:1.5] plot (\x*\x, \x);
								\node at (2,1.75) {$f(x)= \sqrt{x}$};
								%%
								\draw [curve,dashed,samples=100,domain=-1.3:1.3] plot (\x*\x*\x, \x);
								\node at (1,-.5) {$f(x)= \sqrt[3]{x}$};
							\end{tikzpicture}
					</latex-image>
				</image>
				<image width="50%" xml:id="img_graphs3">
					
					<latex-image>
							\begin{tikzpicture}[scale=.5]
								\draw[axes] (-4.8,0) -- (4.8,0);
								\draw[axes] (0,-4.8) -- (0,4.8);		
								%%
								\draw [curve,smooth,samples=100,domain=0:2.2] plot (\x, 2^\x);
								\draw [curve,smooth,samples=100,domain=0:3] plot (-\x, 1/2^\x);
								\node at (3,2) {$f(x)= 2^x$};
								%%
								\draw [curve,dashed,samples=100,domain=0:2] plot (-\x, 2^\x);
								\draw [curve,dashed,samples=100,domain=0:4] plot (\x, 1/2^\x);
								\node at (-3.65,2) {$f(x)= \left(\frac{1}{2}\right)^x$};
							\end{tikzpicture}
					</latex-image>
				</image>
				<image width="50%" xml:id="img_graphs4">
					
					<latex-image>
							\begin{tikzpicture} 
								\draw[axes] (-2.4,0) -- (2.4,0);
								\draw[axes] (0,-2.4) -- (0,2.4);		
								%%
								\draw [curve,smooth,samples=100,domain=1:1.4] plot (\x^3, \x);
								\draw [curve,smooth,samples=100,domain=0:1] plot (\x, \x^2);
								\draw [curve,smooth,samples=100,domain=-2:0] plot (\x, -\x);
								\node at (2.4,-1.1) {$f(x)= \begin{cases} 
										\sqrt[3]x &amp; \text{if }x\geq 1\\
										x^2 &amp; \text{if }1 &gt; x\geq 0\\
										-x &amp; \text{if } x &lt; 0\\		
									\end{cases}
									$};
							\end{tikzpicture}
					</latex-image>
				</image>

		</subsection>

	</section>




</appendix>